RegexCorrectness/NFA.lean
@@ -1,1 +1,3 @@
-import RegexCorrectness.NFA.Correctness
+import RegexCorrectness.NFA.Basic
+import RegexCorrectness.NFA.Compile
+import RegexCorrectness.NFA.Transition
