RegexCorrectness/NFA/Transition/Closure.lean
@@ -1,0 +1,2 @@
+import RegexCorrectness.NFA.Transition.Closure.Basic
+import RegexCorrectness.NFA.Transition.Closure.Equivalence
