RegexCorrectness/NFA/Transition/Path/Equivalence.lean
@@ -1,37 +1,10 @@
 -- Equivalance between a Regex match and a NFA path to the .done node
-import RegexCorrectness.NFA.Transition.Basic
-import RegexCorrectness.NFA.Transition.AcceptOfMatch
-import RegexCorrectness.NFA.Transition.MatchOfAccept
+import RegexCorrectness.NFA.Transition.Path.Equivalence.PathOfMatch
+import RegexCorrectness.NFA.Transition.Path.Equivalence.MatchOfPath
 
-namespace NFA
+namespace Regex.NFA
 
-theorem εClosure_of_pathIn {nfa : NFA} {start} (path : nfa.pathIn start i i' []) :
-  i' ∈ nfa.εClosure i := by
-  generalize h : [] = cs at path
-  induction path with
-  | base _ => exact .base
-  | @step i j k cs cs' step _ ih =>
-    simp at h
-    simp [h] at *
-    cases step with
-    | εStep _ _ step =>
-      exact εClosure.step (εStep_of_εStep step) ih
-
-theorem pathIn_iff_εClosure {nfa : NFA} :
-  nfa.pathIn 0 i i' [] ↔ i' ∈ nfa.εClosure i := by
-  apply Iff.intro
-  . exact εClosure_of_pathIn
-  . intro h
-    induction h with
-    | base => exact .base (Nat.zero_le _)
-    | @step i j k step _ ih =>
-      cases Nat.decLt i nfa.nodes.size with
-      | isTrue lt =>
-        simp [εStep, lt] at step
-        exact .step (.εStep (Nat.zero_le _) lt step) ih
-      | isFalse nlt => simp [εStep, nlt] at step
-
-theorem pathToNext_of_compile_of_pathIn' (eq : NFA.compile r = nfa)
+theorem pathToNext_of_compile_of_pathInAux (eq : NFA.compile r = nfa)
   (assm₁ : 0 < i) (assm₂ : next = 0)
   (path : nfa.pathIn 0 i next cs) :
   nfa.pathToNext 0 1 i cs := by
@@ -64,16 +37,16 @@ theorem pathToNext_of_compile_of_pathIn' (eq : NFA.compile r = nfa)
       have ih := ih this assm₂
       apply ih.cons (step.castStart' assm₁)
 
-theorem pathToNext_of_compile_of_pathIn (eq : NFA.compile r = nfa)
+theorem pathToNext_of_compile_of_pathIn (eq : compile r = nfa)
   (path : nfa.pathIn 0 nfa.start.val 0 cs) :
   nfa.pathToNext 0 1 nfa.start.val cs := by
   have : 0 < nfa.start.val := by
     rw [←eq, compile]
     exact ge_pushRegex_start (rfl : NFA.done.pushRegex _ r = _)
-  exact pathToNext_of_compile_of_pathIn' eq this rfl path
+  exact pathToNext_of_compile_of_pathInAux eq this rfl path
 
-theorem matches_iff_pathToNext {cs : List Char} (eq : NFA.compile r = nfa) :
+theorem matches_iff_pathToNext {cs : List Char} (eq : compile r = nfa) :
   r.matches cs ↔ nfa.pathToNext 0 1 nfa.start.val cs :=
   ⟨pathToNext_of_compile_matches eq, matches_of_pathToNext_compile eq⟩
 
-end NFA
+end Regex.NFA
