RegexCorrectness/NFA/VM.lean
@@ -1,1 +1,0 @@
-import RegexCorrectness.NFA.VM.Traversal
