RegexCorrectness/VM.lean
@@ -1,0 +1,3 @@
+import RegexCorrectness.VM.Auxiliary
+import RegexCorrectness.VM.Basic
+import RegexCorrectness.VM.Correctness
