RegexCorrectness/VM/Correctness.lean
@@ -1,0 +1,18 @@
+import RegexCorrectness.VM.Basic
+
+open Regex.NFA
+
+namespace Regex.VM
+
+theorem matches_of_captureNext
+  (eq : compile re = nfa)
+  (h : captureNext nfa it saveSize = matched)
+  (v : it.Valid)
+  (hsome : matched.isSome) :
+  ∃ (s : Substring) (l m r : List Char),
+    s.ValidFor l m r ∧ it.toString = ⟨l ++ m ++ r⟩ ∧ re.matches m := by
+  have ⟨s, l, m, r, sv, eqs, i, hr, hdone⟩ := captureNext_spec h v hsome
+  have ma := matches_of_reaches eq hr hdone
+  exact ⟨s, l, m, r, sv, eqs, ma⟩
+
+end Regex.VM
